Through to Declarative Typing

theories/NormalForms.v
@@ -1,24 +1,34 @@
 (** * LogRel.NormalForms: definition of normal and neutral forms, and properties. *)
 From LogRel.AutoSubst Require Import core unscoped Ast Extra.
-From LogRel Require Import Utils BasicAst Context.
+From LogRel Require Import Utils BasicAst Context LContexts.
 
 (** ** Weak-head normal forms and neutrals. *)
 
-Inductive whnf : term -> Type :=
+Inductive whne {l : wfLCon} : term -> Type :=
+  | whne_tRel {v} : whne (tRel v)
+  | whne_tApp {n t} : whne n -> whne (tApp n t)
+  | whne_tNatElim {P hz hs n} : whne n -> whne (tNatElim P hz hs n)
+  | whne_tBoolElim {P hz hs n} : whne n -> whne (tBoolElim P hz hs n)
+  | whne_tEmptyElim {P e} : whne e -> whne (tEmptyElim P e)
+  | whne_containsne {t} : containsne t -> whne (tAlpha t)
+with containsne {l : wfLCon} : term -> Type :=
+  | necontne {t}: whne t -> containsne t
+  | scontne {t} : containsne t -> containsne (tSucc t).
+
+Inductive whnf {l : wfLCon} : term -> Type :=
   | whnf_tSort {s} : whnf (tSort s)
   | whnf_tProd {A B} : whnf (tProd A B)
   | whnf_tLambda {A t} : whnf (tLambda A t)
   | whnf_tNat : whnf tNat
   | whnf_tZero : whnf tZero
   | whnf_tSucc {n} : whnf (tSucc n)
+  | whnf_tBool : whnf tBool
+  | whnf_tTrue : whnf tTrue
+  | whnf_tFalse : whnf tFalse
   | whnf_tEmpty : whnf tEmpty
-  | whnf_whne {n} : whne n -> whnf n
-with whne : term -> Type :=
-  | whne_tRel {v} : whne (tRel v)
-  | whne_tApp {n t} : whne n -> whne (tApp n t)
-  | whne_tNatElim {P hz hs n} : whne n -> whne (tNatElim P hz hs n)
-  | whne_tEmptyElim {P e} : whne e -> whne (tEmptyElim P e).
-
+  | whnf_whne {n} : whne (l := l) n -> whnf n
+  | whnf_tAlpha {n} : not_in_LCon (fst l) n -> whnf (tAlpha (nat_to_term n)).
+  
 #[global] Hint Constructors whne whnf : gen_typing.
 
 Ltac inv_whne :=
@@ -27,64 +37,94 @@ Ltac inv_whne :=
     try solve [inversion H] ; block H
   end; unblock.
 
-Lemma neSort s : whne (tSort s) -> False.
+Lemma neSort {l} s : whne (l := l) (tSort s) -> False.
 Proof.
   inversion 1.
 Qed.
 
-Lemma nePi A B : whne (tProd A B) -> False.
+Lemma nePi {l} A B : whne (l := l) (tProd A B) -> False.
 Proof.
   inversion 1.
 Qed.
 
-Lemma neLambda A t : whne (tLambda A t) -> False.
+Lemma neLambda {l} A t : whne (l := l) (tLambda A t) -> False.
 Proof.
   inversion 1.
+Qed.
+
+Lemma containsnewhnf {l} t : containsne (l := l) t -> whnf (l := l) t.
+Proof.
+  intro H.
+  inversion H ; subst.
+  - now eapply whnf_whne.
+  - now eapply whnf_tSucc.
+Qed.
+
+Lemma containsnenattoterm {l} t : containsne (l := l) (nat_to_term t) -> False.
+Proof.
+  intro H.
+  induction t ; cbn in *.
+  - inversion H ; subst.
+    now inversion H0.
+  - inversion H ; subst.
+    + inversion H0.
+    + now eapply IHt.
+Qed.
+
+Lemma whnfnattoterm {l} t : whnf (l := l) (nat_to_term t).
+Proof.
+  induction t  ; cbn.
+  - now econstructor.
+  - now econstructor.
 Qed.
 
 #[global] Hint Resolve neSort nePi neLambda : gen_typing.
 
 (** ** Restricted classes of normal forms *)
 
-Inductive isType : term -> Type :=
+Inductive isType {l} : term -> Type :=
   | UnivType {s} : isType (tSort s)
   | ProdType { A B} : isType (tProd A B)
   | NatType : isType tNat
+  | BoolType : isType tBool
   | EmptyType : isType tEmpty
-  | NeType {A}  : whne A -> isType A.
+  | NeType {A}  : whne (l := l) A -> isType A.
 
-Inductive isPosType : term -> Type :=
+Inductive isPosType {l} : term -> Type :=
   | UnivPos {s} : isPosType (tSort s)
   | NatPos : isPosType tNat
+  | BoolPos : isPosType tBool
   | EmptyPos : isPosType tEmpty
-  | NePos {A}  : whne A -> isPosType A.
+  | NePos {A}  : whne (l := l) A -> isPosType A.
 
-Inductive isFun : term -> Type :=
+Inductive isFun {l} : term -> Type :=
   | LamFun {A t} : isFun (tLambda A t)
-  | NeFun  {f} : whne f -> isFun f.
+  | NeFun  {f} : whne (l := l) f -> isFun f.
 
-Definition isPosType_isType t (i : isPosType t) : isType t :=
+Definition isPosType_isType {l} t (i : isPosType (l := l) t) : isType t :=
   match i with
     | UnivPos => UnivType
     | NatPos => NatType
+    | BoolPos => BoolType
     | EmptyPos => EmptyType
     | NePos ne => NeType ne
   end.
 
 Coercion isPosType_isType : isPosType >-> isType.
 
-Definition isType_whnf t (i : isType t) : whnf t :=
+Definition isType_whnf {l} t (i : isType t) : whnf (l:= l) t :=
   match i with
     | UnivType => whnf_tSort
     | ProdType => whnf_tProd
     | NatType => whnf_tNat
+    | BoolType => whnf_tBool
     | EmptyType => whnf_tEmpty
     | NeType ne => whnf_whne ne
   end.
 
 Coercion isType_whnf : isType >-> whnf.
 
-Definition isFun_whnf t (i : isFun t) : whnf t :=
+Definition isFun_whnf {l} t (i : isFun t) : whnf (l:= l) t :=
   match i with
     | LamFun => whnf_tLambda
     | NeFun ne => whnf_whne ne
