theories/UntypedReduction.v
@@ -1,45 +1,57 @@
 (** * LogRel.UntypedReduction: untyped reduction, used to define algorithmic typing.*)
 From Coq Require Import CRelationClasses.
 From LogRel.AutoSubst Require Import core unscoped Ast Extra.
-From LogRel Require Import Utils BasicAst Notations Context NormalForms Weakening.
+From LogRel Require Import Utils BasicAst Notations Context LContexts NormalForms Weakening.
 
 (** ** Reductions *)
 
 (** *** One-step reduction. *)
 
-Inductive OneRedAlg : term -> term -> Type :=
+Inductive OneRedAlg {l : wfLCon} : term -> term -> Type :=
 | BRed {A a t} :
-    [ tApp (tLambda A t) a ⇒ t[a..] ]
+    [ (tApp (tLambda A t) a) ⇒ t[a..] ]< l >
 | appSubst {t u a} :
-    [ t ⇒ u ] ->
-    [ tApp t a ⇒ tApp u a ]
+    [ t ⇒ u ]< l > ->
+    [ tApp t a ⇒ tApp u a ]< l >
 | natElimSubst {P hz hs n n'} :
-    [ n ⇒ n' ] ->
-    [ tNatElim P hz hs n ⇒ tNatElim P hz hs n' ]
+    [ n ⇒ n' ]< l > ->
+    [ tNatElim P hz hs n ⇒ tNatElim P hz hs n' ]< l >
 | natElimZero {P hz hs} :
-    [ tNatElim P hz hs tZero ⇒ hz ]
+    [ tNatElim P hz hs tZero ⇒ hz ]< l >
 | natElimSucc {P hz hs n} :
-    [ tNatElim P hz hs (tSucc n) ⇒ tApp (tApp hs n) (tNatElim P hz hs n) ]
+  [ tNatElim P hz hs (tSucc n)
+      ⇒ tApp (tApp hs n) (tNatElim P hz hs n) ]< l >
 | termRedEmptyElimAlg {P e e'} :
-    [e ⇒ e'] ->
-    [tEmptyElim P e ⇒ tEmptyElim P e']        
+    [e ⇒ e']< l > ->
+    [tEmptyElim P e ⇒ tEmptyElim P e']< l >        
+| boolElimSubst {P hz hs n n'} :
+    [ n ⇒ n' ]< l > ->
+    [ tBoolElim P hz hs n ⇒ tBoolElim P hz hs n' ]< l >
+| boolElimTrue {P ht hf} :
+    [ tBoolElim P ht hf tTrue ⇒ ht ]< l >
+| boolElimFalse {P ht hf} :
+  [ tBoolElim P ht hf tFalse ⇒ hf ]< l >
+| alphaSubst {n n'} :
+  [ n ⇒ n' ]< l > -> [ tAlpha n ⇒ tAlpha n' ]< l >
+| alphaRed {n b} : in_LCon (fst l) n b ->
+                   [ tAlpha (nat_to_term n) ⇒ bool_to_term b]< l >
 
-where "[ t ⇒ t' ]" := (OneRedAlg t t') : typing_scope.
+where "[ t ⇒ t' ]< l >" := (OneRedAlg (l := l) t t') : typing_scope.
 
 (* Keep in sync with OneRedTermDecl! *)
 
 (** *** Multi-step reduction *)
 
-Inductive RedClosureAlg : term -> term -> Type :=
+Inductive RedClosureAlg {l} : term -> term -> Type :=
   | redIdAlg {t} :
-    [ t ⇒* t ]
+    [ t ⇒* t ]< l >
   | redSuccAlg {t t' u} :
-    [ t ⇒ t'] ->
-    [ t' ⇒* u ] ->
-    [ t ⇒* u ]
-  where "[ t ⇒* t' ]" := (RedClosureAlg t t') : typing_scope.
+    [ t ⇒ t']< l > ->
+    [ t' ⇒* u ]< l > ->
+    [ t ⇒* u ]< l >
+  where "[ t ⇒* t' ]< l >" := (RedClosureAlg (l := l) t t') : typing_scope.
 
-#[export] Instance RedAlgTrans : PreOrder RedClosureAlg.
+#[export] Instance RedAlgTrans {l} : PreOrder (RedClosureAlg (l := l)).
   Proof.
     split.
     - now econstructor.
@@ -56,29 +68,41 @@ Inductive RedClosureAlg : term -> term -> Type :=
 Ltac inv_whne :=
   match goal with [ H : whne _ |- _ ] => inversion H end.
 
-Lemma whne_nored n u :
-  whne n -> [n ⇒ u] -> False.
+Lemma whne_nored {l} n u :
+  whne (l := l) n -> [ n ⇒ u]< l > -> False.
 Proof.
   intros ne red.
   induction red in ne |- *.
   all: inversion ne ; subst ; clear ne.
   2: auto.
-  all: now inv_whne.
+  9: inversion H0 ; subst ; auto; now inversion red.
+  all: try now inv_whne.
+  clear i. induction n ; cbn in *.
+  - inversion H0 ; subst. now inv_whne.
+  - inversion H0 ; subst ; auto. now inv_whne.
 Qed.
 
-Lemma whnf_nored n u :
-  whnf n -> [n ⇒ u] -> False.
+Lemma whnf_nored {l} n u :
+  whnf (l := l) n -> [n ⇒ u]< l > -> False.
 Proof.
   intros nf red.
   induction red in nf |- *.
-  2,3,6: inversion nf; subst; inv_whne; subst; apply IHred; now constructor.
-  all: inversion nf; subst; inv_whne; subst; now inv_whne.
+  2,3,6,7: inversion nf; subst; inv_whne; subst; apply IHred; now constructor.
+  all: inversion nf; subst; try inv_whne; subst; try now inv_whne ; subst.
+  - apply IHred. now eapply containsnewhnf.
+  - apply IHred.
+    now eapply whnfnattoterm.
+  - now eapply containsnenattoterm.
+  - eapply notinLConnotinLCon.
+    exact H0.
+    rewrite (nattoterminj H).
+    exact i.
 Qed.
 
 (** *** Determinism of reduction *)
 
-Lemma ored_det {t u v} :
-  [t ⇒ u] -> [t ⇒ v] ->
+Lemma ored_det {l t u v} :
+  [ t ⇒ u]< l > -> [t ⇒ v]< l > ->
   u = v.
 Proof.
   intros red red'.
@@ -105,9 +129,25 @@ Proof.
     exfalso; eapply whnf_nored; tea; constructor.
   - inversion red'; subst.
     f_equal; eauto.
+  - inversion red'; subst.
+    2,3: exfalso; eapply whnf_nored; tea; constructor.
+    f_equal; eauto.
+  - inversion red'; try reflexivity; subst.
+    exfalso; eapply whnf_nored; tea; constructor.
+  - inversion red'; try reflexivity; subst.
+    exfalso; eapply whnf_nored; tea; constructor.
+  - inversion red' ; subst.
+    + now rewrite (IHred n'0 H0).
+    + exfalso ; eapply whnf_nored ; tea.
+      now eapply whnfnattoterm.
+  - inversion red' ; subst.
+    + exfalso ; eapply whnf_nored ; tea.
+      now eapply whnfnattoterm.
+    + erewrite (uniqueinLCon (snd l) i) ; trivial.
+      rewrite (nattoterminj H) in H0 ; assumption.
 Qed.
 
-Lemma red_whne t u : [t ⇒* u] -> whne t -> t = u.
+Lemma red_whne {l} t u : [t ⇒* u]< l > -> whne (l := l) t -> t = u.
 Proof.
   intros [] ?.
   1: reflexivity.
@@ -115,7 +155,7 @@ Proof.
   eauto using whne_nored.
 Qed.
 
-Lemma red_whnf t u : [t ⇒* u] -> whnf t -> t = u.
+Lemma red_whnf {l} t u : [t ⇒* u]< l > -> whnf (l := l) t -> t = u.
 Proof.
   intros [] ?.
   1: reflexivity.
@@ -123,10 +163,10 @@ Proof.
   eauto using whnf_nored.
 Qed.
 
-Lemma whred_red_det t u u' :
-  whnf u ->
-  [t ⇒* u] -> [t ⇒* u'] ->
-  [u' ⇒* u].
+Lemma whred_red_det {l} t u u' :
+  whnf (l := l) u ->
+  [t ⇒* u]< l > -> [t ⇒* u']< l > ->
+  [u' ⇒* u]< l >.
 Proof.
   intros whnf red red'.
   induction red in whnf, u', red' |- *.
@@ -138,9 +178,9 @@ Proof.
       now eapply IHred.
 Qed.
 
-Corollary whred_det t u u' :
-  whnf u -> whnf u' ->
-  [t ⇒* u] -> [t ⇒* u'] ->
+Corollary whred_det {l} t u u' :
+  whnf (l := l) u -> whnf (l := l) u' ->
+  [t ⇒* u]< l > -> [t ⇒* u']< l > ->
   u = u'.
 Proof.
   intros.
@@ -150,24 +190,28 @@ Qed.
 
 (** *** Stability by weakening *)
 
-Lemma oredalg_wk (ρ : nat -> nat) (t u : term) :
-[t ⇒ u] ->
-[t⟨ρ⟩ ⇒ u⟨ρ⟩].
+Lemma oredalg_wk {l} (ρ : nat -> nat) (t u : term) :
+[t ⇒ u]< l > ->
+[t⟨ρ⟩ ⇒ u⟨ρ⟩]< l >.
 Proof.
   intros Hred.
   induction Hred in ρ |- *.
-  2-5,6: cbn; asimpl; now econstructor.
+  2-5,6,7,8,9,10: cbn; asimpl; now econstructor.
   - cbn ; asimpl.
     evar (t' : term).
     replace (subst_term _ t) with t'.
     all: subst t'.
     1: econstructor.
     now asimpl.
+  - cbn.
+    rewrite <- bool_to_term_ren.
+    rewrite <- nat_to_term_ren.
+    now apply alphaRed.
 Qed.
 
-Lemma credalg_wk (ρ : nat -> nat) (t u : term) :
-[t ⇒* u] ->
-[t⟨ρ⟩ ⇒* u⟨ρ⟩].
+Lemma credalg_wk {l} (ρ : nat -> nat) (t u : term) :
+[t ⇒* u]< l > ->
+[t⟨ρ⟩ ⇒* u⟨ρ⟩]< l >.
 Proof.
   induction 1 ; econstructor ; eauto using oredalg_wk.
 Qed.
